\documentclass[12pt]{article}
\usepackage{pmmeta}
\pmcanonicalname{DerivativesOfsinXAndcosX}
\pmcreated{2013-03-22 16:58:51}
\pmmodified{2013-03-22 16:58:51}
\pmowner{Wkbj79}{1863}
\pmmodifier{Wkbj79}{1863}
\pmtitle{derivatives of $\sin x$ and $\cos x$}
\pmrecord{8}{39257}
\pmprivacy{1}
\pmauthor{Wkbj79}{1863}
\pmtype{Theorem}
\pmcomment{trigger rebuild}
\pmclassification{msc}{26A06}
\pmclassification{msc}{26A09}
\pmclassification{msc}{26A03}
\pmrelated{Derivative2}
\pmrelated{LimitOfDisplaystyleFracsinXxAsXApproaches0}
\pmrelated{LimitOfDisplaystyleFrac1CosXxAsXApproaches0}
\pmrelated{DerivativesOfSineAndCosine}

\endmetadata

\usepackage{amssymb}
\usepackage{amsmath}
\usepackage{amsfonts}

\usepackage{psfrag}
\usepackage{graphicx}
\usepackage{amsthm}
%%\usepackage{xypic}

\newtheorem{thm*}{Theorem}

\begin{document}
\begin{thm*}
$$\frac{d}{dx} (\sin x)=\cos x$$
\end{thm*}

\begin{proof}
\begin{center}
\begin{tabular}{rl}
$\displaystyle \frac{d}{dx} (\sin x)$ & $=\displaystyle \lim_{h \to 0} \frac{\sin (x+h)-\sin x}{h}$ \\
& $=\displaystyle \lim_{h \to 0} \frac{\sin x \cos h+\cos x \sin h-\sin x}{h}$ by addition formula for sine \\
& $=\displaystyle \lim_{h \to 0} \frac{\sin x (\cos h-1)+\cos x \sin h}{h}$ \\
& $=\displaystyle \lim_{h \to 0} \left( \sin x \cdot \frac{\cos h-1}{h} +\cos x \cdot \frac{\sin h}{h} \right)$ \\
& $=\displaystyle \sin x \left( \lim_{h \to 0} \frac{\cos h-1}{h} \right) +\cos x \left( \lim_{h \to 0} \frac{\sin h}{h} \right)$ by \PMlinkname{this entry}{LimitRulesOfFunctions} \\
& $=\displaystyle \sin x \cdot 0+\cos x \cdot 1$ by \PMlinkname{this theorem}{LimitOfDisplaystyleFracsinXxAsXApproaches0} and its \PMlinkname{corollary}{LimitOfDisplaystyleFrac1CosXxAsXApproaches0} \\
& $=\cos x$
\end{tabular}
\end{center}
\end{proof}

\begin{thm*}
$$\frac{d}{dx} (\cos x)=-\sin x$$
\end{thm*}

\begin{proof}
\begin{center}
\begin{tabular}{rl}
$\displaystyle \frac{d}{dx} (\cos x)$ & $=\displaystyle \lim_{h \to 0} \frac{\cos (x+h)-\cos x}{h}$ \\
& $=\displaystyle \lim_{h \to 0} \frac{\cos x \cos h-\sin x \sin h-\cos x}{h}$ by \PMlinkname{addition formula for cosine}{AdditionFormulaForCosine} \\
& $=\displaystyle \lim_{h \to 0} \frac{\cos x (\cos h-1)+\sin x \sin h}{h}$ \\
& $=\displaystyle \lim_{h \to 0} \left( \cos x \cdot \frac{\cos h-1}{h} -\sin x \cdot \frac{\sin h}{h} \right)$ \\
& $=\displaystyle \cos x \left( \lim_{h \to 0} \frac{\cos h-1}{h} \right) -\sin x \left( \lim_{h \to 0} \frac{\sin h}{h} \right)$ by \PMlinkname{this entry}{LimitRulesOfFunctions} \\
& $=\displaystyle \cos x \cdot 0-\sin x \cdot 1$ by \PMlinkname{this theorem}{LimitOfDisplaystyleFracsinXxAsXApproaches0} and its \PMlinkname{corollary}{LimitOfDisplaystyleFrac1CosXxAsXApproaches0} \\
& $=-\sin x$
\end{tabular}
\end{center}
\end{proof}
%%%%%
%%%%%
\end{document}
