\documentclass[12pt]{article}
\usepackage{pmmeta}
\pmcanonicalname{IntegrationOfPolynomial}
\pmcreated{2013-03-22 15:57:29}
\pmmodified{2013-03-22 15:57:29}
\pmowner{Wkbj79}{1863}
\pmmodifier{Wkbj79}{1863}
\pmtitle{integration of polynomial}
\pmrecord{30}{37971}
\pmprivacy{1}
\pmauthor{Wkbj79}{1863}
\pmtype{Theorem}
\pmcomment{trigger rebuild}
\pmclassification{msc}{26A42}

\endmetadata

\usepackage{amssymb}
\usepackage{amsmath}
\usepackage{amsfonts}

\usepackage{psfrag}
\usepackage{graphicx}
\usepackage{amsthm}
%%\usepackage{xypic}

\newtheorem*{thm*}{Theorem}
\begin{document}
\PMlinkescapeword{integral}

\begin{thm*}
For all nonnegative integers $n$,
\[
\int x^n \, dx = \frac{1}{n+1}x^{n+1}+C.
\]
\end{thm*}

\begin{proof}
It will first be proven that, for any nonnegative integer $n$ and any $a \in \mathbb{R}$,
\[
\int\limits_0^a x^n \, dx = \frac{1}{n+1}a^{n+1}.
\]

If $a=0$, the above statement is obvious.  If $a>0$, the following computation uses the right hand rule for computing the \PMlinkname{integral}{RiemannIntegral}; if $a<0$, the following computation uses the left hand rule for computing the integral:

\begin{center}
\begin{tabular}{ll}
$\displaystyle \int\limits_0^a x^n \, dx$ & $\displaystyle =\lim_{t \to \infty} \sum_{k=1}^t \left( \frac{ak}{t} \right)^n \left( \frac{a}{t} \right)$ \\
& $\displaystyle =a^{n+1} \lim_{t \to \infty} \frac{1}{t^{n+1}} \sum_{k=1}^t k^n$ \\
& $\displaystyle =a^{n+1} \lim_{t \to \infty} \frac{1}{t^{n+1}} \sum_{l=1}^{n+1} {n+1 \choose r} \frac{B_{n+1-l}}{n+1}(t+1)^l$ by \PMlinkname{this theorem}{SumOfKthPowersOfTheFirstNPositiveIntegers}, \\
& $\displaystyle =a^{n+1} \lim_{t \to \infty} \frac{1}{t^{n+1}} {n+1 \choose n+1} \frac{B_{n+1-(n+1)}}{n+1} (t+1)^{n+1}$ \\
& $\displaystyle =\frac{B_0}{n+1} a^{n+1} \lim_{t \to \infty} \left( \frac{t+1}{t} \right)^{n+1}$ \\
& $\displaystyle =\frac{1}{n+1}a^{n+1}$ \end{tabular}
\end{center}

Thus, if $a,b \in \mathbb{R}$, then $\displaystyle \int\limits_a^b x^n \, dx = \int\limits_0^b x^n \, dx - \int\limits_0^a x^n \, dx = \frac{1}{n+1}b^{n+1}-\frac{1}{n+1}a^{n+1}.$

It follows that $\displaystyle \int x^n \, dx = \frac{1}{n+1}x^n+C$.
\end{proof}
%%%%%
%%%%%
\end{document}
