\documentclass[12pt]{article}
\usepackage{pmmeta}
\pmcanonicalname{ProofOfMinkowskiInequality}
\pmcreated{2013-03-22 12:42:14}
\pmmodified{2013-03-22 12:42:14}
\pmowner{Andrea Ambrosio}{7332}
\pmmodifier{Andrea Ambrosio}{7332}
\pmtitle{proof of Minkowski inequality}
\pmrecord{10}{32987}
\pmprivacy{1}
\pmauthor{Andrea Ambrosio}{7332}
\pmtype{Proof}
\pmcomment{trigger rebuild}
\pmclassification{msc}{26D15}
\pmrelated{HolderInequality}

% this is the default PlanetMath preamble.  as your knowledge
% of TeX increases, you will probably want to edit this, but
% it should be fine as is for beginners.

% almost certainly you want these
\usepackage{amssymb}
\usepackage{amsmath}
\usepackage{amsfonts}

% used for TeXing text within eps files
%\usepackage{psfrag}
% need this for including graphics (\includegraphics)
%\usepackage{graphicx}
% for neatly defining theorems and propositions
%\usepackage{amsthm}
% making logically defined graphics
%%%\usepackage{xypic}

% there are many more packages, add them here as you need them

% define commands here
\begin{document}
For $p=1$ the result follows immediately from the triangle inequality, so we may assume $p>1$.

We have 
\[ |a_k+b_k|^p=|a_k+b_k| |a_k+b_k|^{p-1} \leq (|a_k|+|b_k|)|a_k+b_k|^{p-1} \]
by the triangle inequality.  Therefore we have 
\[ |a_k+b_k|^p  \leq |a_k||a_k+b_k|^{p-1} + |b_k||a_k+b_k|^{p-1} \]
Set $q=\frac{p}{p-1}$.  Then $\frac{1}{p}+\frac{1}{q}=1$, so by the H\"older inequality we have 
\[ \sum_{k=0}^n |a_k||a_k+b_k|^{p-1} \leq
    \left( \sum_{k=0}^n |a_k|^p \right)^{\frac{1}{p}} 
    \left( \sum_{k=0}^n |a_k+b_k|^{(p-1)q} \right)^{\frac{1}{q}} \]
\[ \sum_{k=0}^n |b_k||a_k+b_k|^{p-1} \leq
    \left( \sum_{k=0}^n |b_k|^p \right)^{\frac{1}{p}} 
    \left( \sum_{k=0}^n |a_k+b_k|^{(p-1)q} \right)^{\frac{1}{q}} \]
Adding these two inequalities, dividing by the factor common to the right sides of both, and observing that $(p-1)q=p$ by definition, we have
\[ \left( \sum_{k=0}^n |a_k+b_k|^p \right)^{1-\frac{1}{q}}
   \leq \frac{ \sum_{k=0}^n (|a_k|+|b_k|)|a_k+b_k|^{p-1} }{ \left( \sum_{k=0}^n |a_k+b_k|^{p} \right)^{\frac{1}{q}} }
   \leq \left( \sum_{k=0}^n |a_k|^p \right)^{\frac{1}{p}} +
        \left( \sum_{k=0}^n |b_k|^p \right)^{\frac{1}{p}}  \]
Finally, observe that $1-\frac{1}{q}=\frac{1}{p}$, and the result follows as required.  The proof for the integral version is analogous.
%%%%%
%%%%%
\end{document}
